compiler_test/beepl_test/BeePL_struct_ex1.v
@@ -1,4 +1,4 @@
-Require Import Integers AST Ctypes BeePL BeeTypes BeePL_values BeePL_typechecker BeePL_Csyntax. 
+Require Import Integers AST Ctypes BeePL BeeTypes BeePL_values BeePL_typechecker BeePL_Csyntax BeePL_notations. 
 From Coq Require Import String ZArith Lists.List.
 From compcert Require Import Csyntaxdefs Errors Maps BeePL_aux.
 Import Csyntaxdefs.CsyntaxNotations.
@@ -9,15 +9,17 @@ Local Open Scope csyntax_scope.
 
 // Define a struct to represent a point in 2D
 struct Point {
-    int x;
-    int y;
+    int *x;
+    int *y;
 };
 
 int main() {
-    struct Point p1;       // Declare a variable of type struct Point
-    p1.x = 10;             // Assign values to fields
-    p1.y = 20;
-    return p1.x;
+    struct Point *p1;       // Declare a variable of type struct Point
+    p1.x := ref 0;
+    p1.y := ref 0;
+    *p1.x := 10;            // Assign values to fields
+    *p1.y := 20;
+    return *p1.x;
 }*)
 
 Definition dattr := {| attr_volatile := false; attr_alignas := None |}.
@@ -26,8 +28,6 @@ Definition _p1 : ident := $"p1".
 Definition _x : ident := $"x".
 Definition _y : ident := $"y".
 Definition _x1 : ident := $"x1".
-Definition _y1 : ident := $"y1".
-Definition _r : ident := $"r".
 Definition _main : ident := $"main".
 
 Definition ident_to_string : list (ident * string) := ((_Point, "Point") ::
@@ -35,36 +35,35 @@ Definition ident_to_string : list (ident * string) := ((_Point, "Point") ::
                                                       (_x, "x") :: 
                                                       (_y, "y") :: 
                                                       (_x1, "x1") ::
-                                                      (_y1, "y1") :: 
-                                                      (_r, "r") ::
                                                       (_main, "main") :: nil).
 
-Definition f_struct : BeePL.function := {| 
-                                   fn_return := (Ptype (BeeTypes.Tint I32 Unsigned dattr));
+(*Definition f_struct : BeePL.function := {| 
+                                   fn_return := tint32u;
                                    fn_effect := nil;
                                    fn_callconv := cc_default;
                                    fn_args := nil;
-                                   fn_vars := ((_p1, BeeTypes.Stype _Point dattr) :: 
-                                               (_x1, (BeeTypes.Ptype (BeeTypes.Tint Ctypes.I32 Ctypes.Unsigned dattr))) ::
-                                               (_y1, (BeeTypes.Ptype (BeeTypes.Tint Ctypes.I32 Ctypes.Unsigned dattr))) ::
-                                               (_r, (Ptype (BeeTypes.Tint I32 Signed dattr))) :: nil);
-                                   fn_body := Bind _x1 (BeeTypes.Ptype (BeeTypes.Tint Ctypes.I32 Ctypes.Unsigned dattr))
-                                                (Prim Massgn ((Sfield (Var _p1 (BeeTypes.Stype _Point dattr)) _x 
-                                                              (BeeTypes.Ptype (BeeTypes.Tint Ctypes.I32 Ctypes.Unsigned dattr))) ::
-                                                              (Const (ConsInt (Int.repr 10)) (Ptype (BeeTypes.Tint I32 Signed dattr))) :: nil)
-                                                              (Ptype Tunit))
-                                                (Bind _y1 (BeeTypes.Ptype (BeeTypes.Tint Ctypes.I32 Ctypes.Unsigned dattr))
-                                                      (Prim Massgn ((Sfield (Var _p1 (BeeTypes.Stype _Point dattr)) _y 
-                                                                    (BeeTypes.Ptype (BeeTypes.Tint Ctypes.I32 Ctypes.Unsigned dattr))) ::
-                                                                    (Const (ConsInt (Int.repr 20)) (Ptype (BeeTypes.Tint I32 Signed dattr))) :: nil)
-                                                      (Ptype Tunit))
-                                                 (Bind _r (BeeTypes.Ptype (BeeTypes.Tint Ctypes.I32 Ctypes.Unsigned dattr))
-                                                  (Sfield (Var _p1 (BeeTypes.Stype _Point dattr)) _x 
-                                                  (BeeTypes.Ptype (BeeTypes.Tint Ctypes.I32 Ctypes.Unsigned dattr)))
-                                                  (Var _r (BeeTypes.Ptype (BeeTypes.Tint Ctypes.I32 Ctypes.Unsigned dattr)))
-                                                  (BeeTypes.Ptype (BeeTypes.Tint Ctypes.I32 Ctypes.Unsigned dattr)))
-                                                (BeeTypes.Ptype (BeeTypes.Tint Ctypes.I32 Ctypes.Unsigned dattr)))
-                                              (BeeTypes.Ptype (BeeTypes.Tint Ctypes.I32 Ctypes.Unsigned dattr)) |}.
+                                   fn_vars := ((_p1, tstruct _Point) :: 
+                                               (_x1, trint32u) :: nil);
+                                   fn_body := Bind _x1 tunit
+                                                (Prim Massgn ((Sfield (Var _p1 (tstruct _Point)) _x trint32u) ::
+                                                              (Prim Ref (cint (Int.repr 0) tint32u :: nil) trint32u) :: nil)
+                                                              tunit)
+                                                (Bind _x1 tunit
+                                                   (Prim Massgn ((Sfield (Var _p1 (tstruct _Point)) _y trint32u) ::
+                                                                 (Prim Ref (cint (Int.repr 0) tint32u :: nil) trint32u) :: nil) tunit)
+                                                   (Bind _x1 tunit 
+                                                      (Prim Massgn (Prim Deref ((Sfield (Var _p1 (tstruct _Point)) _x trint32u) :: nil) trint32u ::
+                                                                    (cint (Int.repr 10) tint32u) :: nil) tunit)
+                                                      (Bind _x1 tunit 
+                                                         (Prim Massgn (Prim Deref ((Sfield (Var _p1 (tstruct _Point)) _y trint32u) :: nil) trint32u ::
+                                                                      (cint (Int.repr 20) tint32u) :: nil) tunit)
+                                                         (Prim Deref ((Sfield (Var _p1 (tstruct _Point)) _x trint32u) :: nil) tint32u)
+                                                         tint32u)
+                                                      tint32u)
+                                                   tint32u)
+                                              tint32u
+
+                                  |}.
 
 Definition global_definitions : list (ident * AST.globdef BeePL.fundef type) 
    := (_main, AST.Gfun(BeePL.Internal (f_struct))) :: nil.
@@ -73,16 +72,29 @@ Definition public_idents : list ident := (_main :: nil).
 
 Definition bcomposites : list bcomposite_definition :=
 (Bcomposite _Point Struct
-   (Member_plain _x (BeeTypes.Ptype (BeeTypes.Tint Ctypes.I32 Ctypes.Unsigned dattr)) :: 
-    Member_plain _y (BeeTypes.Ptype (BeeTypes.Tint Ctypes.I32 Ctypes.Unsigned dattr)) :: nil)
+   (Member_plain _x trint32u :: 
+    Member_plain _y trint32u :: nil)
    noattr :: nil).
 
 Lemma bcomposite_correct :
   wf_bcomposites bcomposites.
 Proof.
   unfold wf_bcomposites.
-  unfold build_bcomposite_env; simpl; constructor. 
-Qed.
+  unfold build_bcomposite_env; simpl; constructor.
+Qed. *)
+
+(*Definition example1 : BeePL.program := @mkbprogram bcomposites 
+                                                   global_definitions 
+                                                   public_idents 
+                                                   _main 
+                                                   bcomposite_correct
+                                                   ident_to_string.*)
+
+(*Compute (type_check_expr beepl_ef_env example1.(prog_comp_env) 
+                         (bind_vars (bind_vars empty_context f_struct.(fn_args)) f_struct.(fn_vars)) empty_context f_struct.(fn_body)).
+
+Compute (type_check_program example1). *) (* Type checks *)
+
 
 (*Definition example1 : BeePL.program := @mkbprogram bcomposites global_definitions public_idents _main bcomposite_correct.
 
