compiler_test/beepl_test/BeePL_struct_ex2.v
@@ -1,21 +1,25 @@
-Require Import Integers AST Ctypes BeePL BeeTypes BeePL_values BeePL_typechecker BeePL_Csyntax. 
+Require Import Integers AST Ctypes BeePL BeeTypes BeePL_values BeePL_typechecker BeePL_Csyntax BeePL_notations. 
 From Coq Require Import String ZArith Lists.List.
 From compcert Require Import Csyntaxdefs Errors Maps BeePL_aux.
 Import Csyntaxdefs.CsyntaxNotations.
 Local Open Scope string_scope.
 Local Open Scope csyntax_scope.
 
-(* #include <stdio.h>
+(*
+#include <stdio.h>
 
 // Define a struct to represent a point in 2D
 struct Point {
-    int x;
-    int y;
+    int *x;
+    int *y;
 };
 
-int main() {
-    struct Point p1;       // Declare a variable of type struct Point
-    return p1.x;
+int main(void)
+{
+  struct Point p1;
+  *p1.x = 10U;
+  return *p1.x;
+}
 }*)
 
 Definition dattr := {| attr_volatile := false; attr_alignas := None |}.
@@ -23,22 +27,27 @@ Definition _Point : ident := $"Point".
 Definition _p1 : ident := $"p1".
 Definition _x : ident := $"x".
 Definition _y : ident := $"y".
+Definition _t : ident := $"t".
+Definition _p2 : ident := $"p2".
 Definition _main : ident := $"main".
 
 Definition ident_to_string : list (ident * string) := ((_Point, "Point") ::
                                                       (_p1, "p1") ::
+                                                      (_p2, "p2") ::
                                                       (_x, "x") :: 
-                                                      (_y, "y") :: 
+                                                      (_y, "y") ::
+                                                      (_t, "t") ::
                                                       (_main, "main") :: nil).
-Definition f_struct : BeePL.function := {| 
-                                   fn_return := (Ptype (BeeTypes.Tint I32 Unsigned dattr));
-                                   fn_effect := nil;
-                                   fn_callconv := cc_default;
-                                   fn_args := nil;
-                                   fn_vars := ((_p1, BeeTypes.Stype _Point dattr) :: nil);
-                                   fn_body := (Sfield (Var _p1 (BeeTypes.Stype _Point dattr)) _x 
-                                                (BeeTypes.Ptype (BeeTypes.Tint Ctypes.I32 Ctypes.Unsigned dattr)))
-                                                |}.
+
+Definition f_struct : BeePL.function := {| fn_return := tint32s;
+                                           fn_effect :=  Write mem_ident :: Read mem_ident :: nil;
+                                           fn_callconv := cc_default;
+                                           fn_args := nil;
+                                           fn_vars := ((_p1, (Reftype mem_ident (Bstruct _Point noattr) noattr)) :: nil);  (* p1 is a struct variable on stack *)
+                                           fn_body := Screate _p1 ((_x, (cint (Int.repr 10) tint32s)) :: (_y, (cint (Int.repr 20) tint32s)) :: nil) 
+                                                        (Reftype mem_ident (Bstruct _Point noattr) noattr)
+                                                       |}.
+                                                      
 
 Definition global_definitions : list (ident * AST.globdef BeePL.fundef type) 
    := (_main, AST.Gfun(BeePL.Internal (f_struct))) :: nil.
@@ -47,8 +56,8 @@ Definition public_idents : list ident := (_main :: nil).
 
 Definition bcomposites : list bcomposite_definition :=
 (Bcomposite _Point Struct
-   (Member_plain _x (BeeTypes.Ptype (BeeTypes.Tint Ctypes.I32 Ctypes.Unsigned dattr)) :: 
-    Member_plain _y (BeeTypes.Ptype (BeeTypes.Tint Ctypes.I32 Ctypes.Unsigned dattr)) :: nil)
+   (Member_plain _x tint32s :: 
+    Member_plain _y tint32s :: nil)
    noattr :: nil).
 
 Lemma bcomposite_correct :
@@ -58,80 +67,17 @@ Proof.
   unfold build_bcomposite_env; simpl; constructor. 
 Qed.
 
-Definition example1 : BeePL.program := @mkbprogram bcomposites global_definitions public_idents _main bcomposite_correct ident_to_string.
+(*Definition example1 : BeePL.program := @mkbprogram bcomposites 
+                                                   global_definitions 
+                                                   public_idents 
+                                                   _main 
+                                                   bcomposite_correct
+                                                   ident_to_string.
 
-(*Compute (type_check_program example1). 
+Compute (type_check_expr example1.(prog_comp_env) 
+                         (bind_vars (bind_vars empty_context f_struct.(fn_args)) f_struct.(fn_vars)) empty_context f_struct.(fn_body)).
 
-Compute (BeePL_Csyntax.BeePL_compcert example1).*)
-
-(*   = OK
-         {|
-           Ctypes.prog_defs :=
-             (22880918%positive,
-             Gfun
-               (Ctypes.Internal
-                  {|
-                    Csyntax.fn_return :=
-                      Ctypes.Tint I32 Unsigned {| attr_volatile := false; attr_alignas := None |};
-                    Csyntax.fn_callconv :=
-                      {| cc_vararg := None; cc_unproto := false; cc_structret := false |};
-                    Csyntax.fn_params := nil;
-                    Csyntax.fn_vars :=
-                      (4185%positive,
-                      Tstruct 1566385715%positive
-                        {| attr_volatile := false; attr_alignas := None |}) :: nil;
-                    Csyntax.fn_body :=
-                      Csyntax.Sdo
-                        (Csyntax.Evalof
-                           (Csyntax.Efield
-                              (Csyntax.Evalof
-                                 (Csyntax.Evar 4185%positive
-                                    (Tstruct 1566385715%positive
-                                       {| attr_volatile := false; attr_alignas := None |}))
-                                 (Tstruct 1566385715%positive
-                                    {| attr_volatile := false; attr_alignas := None |}))
-                              97%positive
-                              (Ctypes.Tint I32 Unsigned
-                                 {| attr_volatile := false; attr_alignas := None |}))
-                           (Ctypes.Tint I32 Unsigned
-                              {| attr_volatile := false; attr_alignas := None |}))
-                  |})) :: nil;
-           Ctypes.prog_public := 22880918%positive :: nil;
-           Ctypes.prog_main := 22880918%positive;
-           Ctypes.prog_types :=
-             Composite 1566385715%positive Struct
-               (Ctypes.Member_plain 97%positive
-                  (Ctypes.Tint I32 Unsigned {| attr_volatile := false; attr_alignas := None |})
-                :: Ctypes.Member_plain 98%positive
-                     (Ctypes.Tint I32 Unsigned {| attr_volatile := false; attr_alignas := None |})
-                   :: nil) {| attr_volatile := false; attr_alignas := None |} :: nil;
-           Ctypes.prog_comp_env :=
-             PTree.Nodes
-               (PTree.Node001
-                  (PTree.Node001
-                     (PTree.Node100
-                        (PTree.Node100
-                           (PTree.Node001
-                              (PTree.Node001
-                                 (PTree.Node100
-                                    (PTree.Node100
-                                       (PTree.Node100
-                                          (PTree.Node001
-                                             (PTree.Node001
-                                                (PTree.Node100
-                                                   (PTree.Node100
-                                                      (PTree.Node001
-                                                         (PTree.Node100
-                                                            (PTree.Node100
-                                                               (PTree.Node001
-                                                                  (PTree.Node100
-                                                                     (PTree.Node001
-                                                                     (PTree.Node001
-                                                                     (PTree.Node001 ...)))))))))))))))))))));
-           Ctypes.prog_comp_env_eq := eq_refl
-         |}
-     : res (Ctypes.program Csyntax.function)
+Compute (type_check_program example1). *)
 
 
-*)
 
